un-hardcode # of reductions

src/Experiments/SimplyTypedArithmetic.v
@@ -1617,16 +1617,19 @@ Module Rows.
         let pq_a := Associational.sat_mul base p_a q_a in
         flatten m (from_associational m pq_a).
 
+      (* TODO : move sat_reduce and repeat_sat_reduce to Saturated.Associational *)
       Definition sat_reduce base s c (p : list (Z * Z)) :=
         let lo_hi := Associational.split s p in
         fst lo_hi ++ (Associational.sat_mul_const base c (snd lo_hi)).
 
-      (* TODO : hardcoded to 2 reductions; fix *)
-      Definition mulmod base s c n (p q : list Z) :=
+      Definition repeat_sat_reduce base s c (p : list (Z * Z)) n :=
+        fold_right (fun _ q => sat_reduce base s c q) p (seq 0 n).
+
+      Definition mulmod base s c n nreductions (p q : list Z) :=
         let p_a := Positional.to_associational weight n p in
         let q_a := Positional.to_associational weight n q in
         let pq_a := Associational.sat_mul base p_a q_a in
-        let r_a := sat_reduce base s c (sat_reduce base s c pq_a) in
+        let r_a := repeat_sat_reduce base s c pq_a nreductions in
         flatten n (from_associational n r_a).
 
       Hint Rewrite Associational.eval_sat_mul_const Associational.eval_sat_mul Associational.eval_split using solve [auto] : push_eval.
@@ -1677,19 +1680,38 @@ Module Rows.
         fst (mul base n m p q) = partition m (Positional.eval weight n p * Positional.eval weight n q).
       Proof. solver. Qed.
 
-      Lemma eval_mulmod base s c n p q :
+      Lemma eval_sat_reduce base s c p :
+        base <> 0 -> s - Associational.eval c <> 0 -> s <> 0 ->
+        Associational.eval (sat_reduce base s c p) mod (s - Associational.eval c)
+        = Associational.eval p mod (s - Associational.eval c).
+      Proof.
+        intros; cbv [sat_reduce].
+        autorewrite with push_eval.
+        rewrite <-Associational.reduction_rule by omega.
+        autorewrite with push_eval; reflexivity.
+      Qed.
+      Hint Rewrite eval_sat_reduce using auto : push_eval.
+
+      Lemma eval_repeat_sat_reduce base s c p n :
+        base <> 0 -> s - Associational.eval c <> 0 -> s <> 0 ->
+        Associational.eval (repeat_sat_reduce base s c p n) mod (s - Associational.eval c)
+        = Associational.eval p mod (s - Associational.eval c).
+      Proof.
+        intros; cbv [repeat_sat_reduce].
+        apply fold_right_invariant; intros; autorewrite with push_eval; auto.
+      Qed.
+      Hint Rewrite eval_repeat_sat_reduce using auto : push_eval.
+
+      Lemma eval_mulmod base s c n nreductions p q :
         base <> 0 -> s <> 0 -> s - Associational.eval c <> 0 ->
         n <> 0%nat -> length p = n -> length q = n ->
-        (Positional.eval weight n (fst (mulmod base s c n p q))
-         + weight n * (snd (mulmod base s c n p q))) mod (s - Associational.eval c)
+        (Positional.eval weight n (fst (mulmod base s c n nreductions p q))
+         + weight n * (snd (mulmod base s c n nreductions p q))) mod (s - Associational.eval c)
         = (Positional.eval weight n p * Positional.eval weight n q) mod (s - Associational.eval c).
       Proof.
         solver.
         rewrite <-Z.div_mod'' by auto.
-        rewrite <-Associational.reduction_rule by omega.
-        autorewrite with push_eval.
-        rewrite <-Associational.reduction_rule by omega.
-        autorewrite with push_eval; auto.
+        autorewrite with push_eval; reflexivity.
       Qed.
     End Ops.
   End Rows.
@@ -8478,7 +8500,7 @@ Module SaturatedSolinas.
     Context (s : Z) (c : list (Z * Z))
             (s_nz : s <> 0) (modulus_nz : s - Associational.eval c <> 0).
     Context (log2base : Z) (log2base_pos : 0 < log2base)
-            (n : nat) (n_nz : n <> 0%nat).
+            (n nreductions : nat) (n_nz : n <> 0%nat).
 
     Let weight := weight log2base 1.
     Let props : @weight_properties weight := wprops log2base 1 ltac:(omega).
@@ -8493,7 +8515,7 @@ Module SaturatedSolinas.
            As eval_mulmod.
     Proof.
       intros.
-      rewrite <-Rows.eval_mulmod with (base:=2^log2base) (s:=s) (c:=c) by auto using base_nz.
+      rewrite <-Rows.eval_mulmod with (base:=2^log2base) (s:=s) (c:=c) (nreductions:=nreductions) by auto using base_nz.
       eapply f_equal2; [|trivial].
       (* expand_lists (). *) (* uncommenting this line removes some unused multiplications but also inlines a bunch of carry stuff at the end *)
       subst mulmod. reflexivity.
@@ -8502,15 +8524,15 @@ Module SaturatedSolinas.
   End MulMod.
 
   Derive mulmod_gen
-         SuchThat (forall (log2base s : Z) (c : list (Z * Z)) (n m : nat)
+         SuchThat (forall (log2base s : Z) (c : list (Z * Z)) (n nreductions : nat)
                           (f g : list Z),
                       Interp (t:=type.reify_type_of mulmod')
-                             mulmod_gen s c log2base n f g
-                      = mulmod' s c log2base n f g)
+                             mulmod_gen s c log2base n nreductions f g
+                      = mulmod' s c log2base n nreductions f g)
          As mulmod_gen_correct.
   Proof. Time cache_reify (). exact admit. (* correctness of initial parts of the pipeline *) Time Qed.
   Module Export ReifyHints.
-    Global Hint Extern 1 (_ = mulmod' _ _ _ _ _ _) => simple apply mulmod_gen_correct : reify_gen_cache.
+    Global Hint Extern 1 (_ = mulmod' _ _ _ _ _ _ _) => simple apply mulmod_gen_correct : reify_gen_cache.
   End ReifyHints.
 
   Section rmulmod.
@@ -8521,7 +8543,15 @@ Module SaturatedSolinas.
     Definition relax_zrange_of_machine_wordsize
       := relax_zrange_gen [1; machine_wordsize]%Z.
 
-    Let n : nat := Z.to_nat (Z.log2 s / machine_wordsize).
+    Let n : nat := Z.to_nat (Qceiling (Z.log2_up s / machine_wordsize)).
+    (* Number of reductions is calculated as follows :
+         Let i be the highest limb index of c. Then, each reduction
+         decreases the number of extra limbs by (n-i). So, to go from
+         the n extra limbs we have post-multiplication down to 0, we
+         need ceil (n / (n - i)) reductions. *)
+    Let nreductions : nat :=
+      let i := fold_right Z.max 0 (map (fun t => Z.log2 (fst t) / machine_wordsize) c) in
+      Z.to_nat (Qceiling (Z.of_nat n / (Z.of_nat n - i))).
     Let relax_zrange := relax_zrange_of_machine_wordsize.
     Let bound := Some r[0 ~> (2^machine_wordsize - 1)]%zrange.
     Let boundsn : list (ZRange.type.option.interp type.Z)
@@ -8563,7 +8593,7 @@ Module SaturatedSolinas.
     := BoundsPipeline_correct
          (Some boundsn, Some boundsn)
          (Some boundsn)
-         (mulmod' s c machine_wordsize n).
+         (mulmod' s c machine_wordsize n nreductions).
 
     Notation type_of_strip_3arrow := ((fun (d : Prop) (_ : forall A B C, d) => d) _).
     Definition rmulmod_correctT rv : Prop
@@ -8839,6 +8869,8 @@ mulmod = fun var : type -> Type => λ x : var (type.list (type.type_primitive ty
 
 End P192_32.
 
+(* TODO : Too slow! Many, many terms in this one. *)
+(*
 Module P256_32.
   Definition s := 2^256.
   Definition c :=  [(2^224, 1); (2^192, -1); (2^96, -1); (1,1)].
@@ -8854,14 +8886,9 @@ Module P256_32.
   Set Printing Width 100000.
 
   Print mulmod.
-  (* TODO : this one should use more reductions *)
-  (* Since 224 = 7*32, first reduce will leave 7 extra words
-     Each reduce changes that number by only 1
-     therefore we need 8 reductions
-   *)
-
 
 End P256_32.
+*)
 
 Module MontgomeryReduction.
   Section MontRed'.
